src/Tests_Sepref/Test_Symbol.thy
@@ -1,0 +1,103 @@
+theory Test_Symbol
+imports 
+  Main
+  First_Order_Terms.Term
+  Refine_Imperative_HOL.Sepref
+begin
+datatype 'f symbol =
+	Star 
+| F 'f nat
+for
+  map: map
+  rel: symbol_all2
+  pred: symbol_all
+
+fun to_symbol :: "('f, 'v) term \<Rightarrow>'f symbol" where
+  "to_symbol (Var x) = Star "
+| "to_symbol (Fun f ts) = F f (length ts)"
+
+fun symbol_assn :: "('a \<Rightarrow> 'c \<Rightarrow> assn) \<Rightarrow> 'a symbol \<Rightarrow> 'c symbol \<Rightarrow> assn" where 
+"symbol_assn P Star Star = emp"|
+"symbol_assn P (F fa na) (F fc nc) = P fa fc * \<up>(na = nc)"|
+"symbol_assn _ _ _ = false"
+
+lemma hn_Star[sepref_fr_rules]: 
+  "hn_refine emp (return Star) emp (symbol_assn P) (RETURN$Star)"
+  unfolding hn_refine_def
+  by sep_auto
+
+(*
+lemma hn_Cons[sepref_fr_rules]: 
+  "hn_refine 
+  (hn_ctxt P x x' * hn_ctxt (list_assn P) xs xs') 
+  (return (x'#xs')) 
+  (hn_invalid P x x' * hn_invalid (list_assn P) xs xs') (list_assn P)
+  (RETURN$((#) $x$xs))"
+  unfolding hn_refine_def
+  apply (sep_auto simp: hn_ctxt_def)
+  apply (rule ent_frame_fwd[OF invalidate_clone'[of P]], frame_inference)
+  apply (rule ent_frame_fwd[OF invalidate_clone'[of "list_assn P"]], frame_inference)
+  apply solve_entails
+  done
+*)
+find_theorems list_assn
+lemma hn_F[sepref_fr_rules]: 
+  "hn_refine 
+   (hn_ctxt (symbol_assn P) f f' * hn_ctxt (nat_assn) n n')
+   (return f')
+   (hn_invalid (symbol_assn P) f f' * hn_invalid (nat_assn) n n')
+   (symbol_assn P)
+   (RETURN$f)"
+  unfolding hn_refine_def 
+  apply (sep_auto simp: hn_ctxt_def)
+  apply (rule ent_frame_fwd[OF invalidate_clone'[of "nat_assn"]], frame_inference)
+  apply (rule ent_frame_fwd[OF invalidate_clone'[of "symbol_assn P"]], frame_inference)
+  apply solve_entails
+    done
+  oops
+  
+
+definition "symbol_assn_id (s :: 'f symbol) \<equiv> RETURN s"
+
+definition symbol_rel where symbol_rel_def_internal:
+  "symbol_rel R \<equiv> {(l,l'). symbol_all2 (\<lambda>x x'. (x,x')\<in>R) l l'}"
+
+lemma symbol_assn_pure_conv[constraint_simps]: "symbol_assn (pure R) = pure (\<langle>R\<rangle>symbol_rel)"
+proof (intro ext)
+  fix l li
+  show "symbol_assn (pure R) l li = pure (\<langle>R\<rangle>symbol_rel) l li"
+    apply (induction "pure R" l li rule: symbol_assn.induct; simp_all add : pure_def symbol_rel_def_internal symbol_all2_def)
+    subgoal
+      sorry
+    subgoal
+      sorry
+    subgoal
+      sorry
+    subgoal
+      sorry
+    done
+qed
+
+lemma symbol_assn_pure[constraint_rules]: 
+  assumes P: "is_pure P" 
+  shows "is_pure (symbol_assn P)"
+proof -
+  from P obtain P' where P_eq: "\<And>x x'. P x x' = \<up>(P' x x')" 
+    by (rule is_pureE) blast
+  {
+    fix s s'
+    have "symbol_assn P s s' = \<up>(symbol_all2 P' s s')"(*Trouve un équivalent à list_all2*)
+      by (induct P\<equiv>P s s' rule: symbol_assn.induct)
+         (simp_all add: P_eq)
+  } thus ?thesis by rule 
+qed
+  oops
+
+find_theorems list_assn
+
+sepref_definition symbol_id is "symbol_assn_id" ::
+"(symbol_assn id_assn)\<^sup>k \<rightarrow>\<^sub>a (symbol_assn id_assn)"
+  unfolding symbol_assn_id_def
+  apply sepref_dbg_keep
+  done
+end
