src/Tests_Sepref/Test_Tree.thy
@@ -33,6 +33,7 @@ fun tree_assn :: "('a \<Rightarrow> 'c \<Rightarrow> assn) \<Rightarrow> 'a tree
 "tree_assn P (Node va la ra) (Node vc lc rc) = P va vc * tree_assn P la lc * tree_assn P ra rc" |
 "tree_assn _ _ _ = false"
 
+
 definition tree_rel where tree_rel_def_internal:
   "tree_rel R \<equiv> {(t,t'). tree_all2 (\<lambda>x x'. (x,x')\<in>R) t t'}"
 
@@ -76,12 +77,22 @@ proof (intro ext)
     apply (induction "pure R" t ti rule: tree_assn.induct)
     by (simp_all add: pure_def tree_rel_def)
 qed
-lemma tree_match_cong[sepref_frame_match_rules]: 
-  "\<lbrakk>\<And>x x'. \<lbrakk>x\<in>set t; x'\<in>set t'\<rbrakk> \<Longrightarrow> hn_ctxt A x x' \<Longrightarrow>\<^sub>t hn_ctxt A' x x' \<rbrakk> \<Longrightarrow> hn_ctxt (tree_assn A) t t' \<Longrightarrow>\<^sub>t hn_ctxt (tree_assn A') t t'"
-  unfolding hn_ctxt_def
-  by (induct A t t' rule: tree_assn.induct) (simp_all add: entt_star_mono)
+lemma tree_assn_pure[constraint_rules]: 
+  assumes P: "is_pure P" 
+  shows "is_pure (tree_assn P)"
+proof -
+  from P obtain P' where P_eq: "\<And>x x'. P x x' = \<up>(P' x x')" 
+    by (rule is_pureE) blast
 
+  {
+    fix l l'
+    have "tree_assn P l l' = \<up>(tree_all2 P' l l')"
+      by (induct P\<equiv>P l l' rule: tree_assn.induct)
+         (simp_all add: P_eq)
+  } thus ?thesis by rule
+qed
 lemmas hn_ctxt_tree = hn_ctxt_eq[of "tree_assn A" for A]
+
 
 lemma hn_case_tree[sepref_prep_comb_rule, sepref_comb_rules, simp]:
   fixes p p' P
@@ -163,7 +174,6 @@ lemma tree_case_hnr[simplified mult.commute mult.assoc]:
     done
   done
 
-
 lemma hn_Leaf[sepref_fr_rules]: 
   "hn_refine emp (return Leaf) emp (tree_assn P) (RETURN$Leaf)"
   unfolding hn_refine_def
@@ -178,23 +188,9 @@ lemma hn_Cons[sepref_fr_rules]:
   apply (rule ent_frame_fwd[OF invalidate_clone'[of P]], frame_inference)
   apply (rule ent_frame_fwd[OF invalidate_clone'[of "tree_assn P"]], frame_inference) 
   by (smt (verit) assn_aci(10) assn_times_comm ent_true_drop(1) invalid_assn_def invalidate lambda_one mult.right_neutral
-      prec_split1_aux pure_false pure_true star_false_right)
+      prec_split1_aux pure_false pure_true star_false_right)  
   
-  
-lemma tree_assn_pure[constraint_rules]: 
-  assumes P: "is_pure P" 
-  shows "is_pure (tree_assn P)"
-proof -
-  from P obtain P' where P_eq: "\<And>x x'. P x x' = \<up>(P' x x')" 
-    by (rule is_pureE) blast
 
-  {
-    fix l l'
-    have "tree_assn P l l' = \<up>(tree_all2 P' l l')"
-      by (induct P\<equiv>P l l' rule: tree_assn.induct)
-         (simp_all add: P_eq)
-  } thus ?thesis by rule
-qed
 
 find_theorems list_assn
 
