src/Tests_Sepref/Test_nres.thy
@@ -1,0 +1,51 @@
+theory Test_nres
+
+imports 
+  Main
+  First_Order_Terms.Term
+  Refine_Imperative_HOL.IICF
+  Refine_Imperative_HOL.Sepref
+  "Finite-Map-Extras.Finite_Map_Extras"
+
+begin
+
+
+datatype 'f symbol =
+	Star 
+| F 'f nat
+
+
+datatype (plugins del: size) ('f,'v) trie =
+  Leaf "('f,'v) term set"
+| SymbolNode (children: "('f symbol, (nat, ('f, 'v) trie) fmap) fmap")
+  where
+    "children (Leaf x) = fmempty"
+
+function (domintros) trie_depth :: "('f,'v) trie \<Rightarrow> nat" where
+  "trie_depth (Leaf ts)       = 1"
+| "trie_depth (SymbolNode m) = Suc (Max (trie_depth ` \<Union> (fmran' ` (fmran' m))))"
+  by pat_completeness auto
+termination
+proof -
+  have "\<And>x. trie_depth_dom x"
+  proof -
+    fix x :: "('f ,'v) trie"
+    show "trie_depth_dom x"
+    proof (induction x)
+      case (Leaf ts)
+      then show ?case using trie_depth.domintros(1) by blast
+    next
+      case (SymbolNode m)
+      then show ?case using trie_depth.domintros(2) by blast
+    qed
+  qed
+  then show ?thesis by auto
+qed
+
+function trie_depth_nres :: "('f,'v) trie \<Rightarrow> nat nres" where
+"trie_depth_nres t \<equiv> do(RETURN 0)"
+
+
+
+end
+
